src/program_proof/memkv/memkv_conditional_put_proof.v
@@ -1,0 +1,514 @@
+From Perennial.program_proof Require Import dist_prelude.
+From Goose.github_com.mit_pdos.gokv Require Import memkv.
+From Perennial.program_proof.lockservice Require Import rpc.
+From Perennial.program_proof.memkv Require Export memkv_shard_definitions common_proof.
+
+Section memkv_conditional_put_proof.
+
+Context `{!heapG Σ, rpcG Σ ShardReplyC, HREG: rpcregG Σ, kvMapG Σ}.
+
+Local Ltac Zify.zify_post_hook ::= Z.div_mod_to_equations.
+
+(* FIXME: move somewhere mor general *)
+Lemma wp_If_join_evar (b : bool) e1 e2 Q Φ :
+  (∀ b', ⌜b' = b⌝ -∗ WP if: #b then e1 else e2 {{ v, ⌜v = #()⌝ ∗ Q b' }}) -∗
+  (Q b -∗ Φ #()) -∗ WP if: #b then e1 else e2 {{ Φ }}.
+Proof.
+  iIntros "Hif Hcont". iApply (wp_wand with "[Hif]").
+  - iApply "Hif". done.
+  - simpl. iIntros (v) "[-> HQ]". by iApply "Hcont".
+Qed.
+
+Lemma wp_ConditionalPutRPC (s args_ptr reply_ptr:loc) expv_sl newv_sl args γ Eo Ei γreq Q :
+  is_MemKVShardServer s γ -∗
+  {{{
+       own_ConditionalPutRequest args_ptr expv_sl newv_sl args ∗
+       (∃ dummy_rep, own_ConditionalPutReply reply_ptr dummy_rep) ∗
+       is_RPCRequest γ.(rpc_gn) γreq (PreShardConditionalPut Eo Ei γ args.(CPR_Key) Q args.(CPR_ExpValue) args.(CPR_NewValue))
+                                (PostShardConditionalPut Eo Ei γ args.(CPR_Key) Q args.(CPR_ExpValue) args.(CPR_NewValue))
+                                {| Req_CID:=args.(CPR_CID); Req_Seq:=args.(CPR_Seq) |}
+  }}}
+    MemKVShardServer__ConditionalPutRPC #s #args_ptr #reply_ptr
+  {{{
+       rep, RET #();
+       own_ConditionalPutReply reply_ptr rep ∗
+       (RPCRequestStale γ.(rpc_gn) {| Req_CID:=args.(CPR_CID); Req_Seq:=args.(CPR_Seq) |} ∨
+        ∃ dummy_val, RPCReplyReceipt γ.(rpc_gn) {| Req_CID:=args.(CPR_CID); Req_Seq:=args.(CPR_Seq) |} (mkShardReplyC rep.(CPR_Err) dummy_val rep.(CPR_Succ)))
+  }}}.
+Proof.
+  iIntros "#His_shard !#" (Φ) "Hpre HΦ".
+  iDestruct "Hpre" as "(Hargs & Hrep & #HreqInv)".
+  iNamed "Hargs". iNamed "Hrep".
+
+  wp_lam.
+  wp_pures.
+
+  iNamed "His_shard".
+  wp_loadField.
+  wp_apply (acquire_spec with "[$HmuInv]").
+  iIntros "[Hlocked Hown]".
+
+  iNamed "Hown".
+
+  wp_pures.
+  wp_lam.
+  wp_pures.
+
+  wp_loadField. wp_loadField.
+  wp_apply (wp_MapGet with "HlastSeqMap").
+  iIntros (seqno ok) "[%HseqGet HlastSeqMap]".
+  wp_pures.
+
+  wp_loadField.
+  wp_pures.
+
+  wp_apply (wp_and ok (int.Z args.(CPR_Seq) ≤ int.Z seqno)%Z).
+  { wp_pures. by destruct ok. }
+  { iIntros "_". wp_pures. done. }
+
+  wp_if_destruct.
+  { (* reply table *)
+    wp_loadField.
+    wp_loadField.
+    wp_apply (map.wp_MapGet with "HlastReplyMap").
+    iIntros (reply replyOk) "[%HlookupReply HlastReplyMap]".
+    wp_pures.
+    Transparent struct.store.
+    unfold struct.store.
+    Opaque struct.store.
+    Opaque struct.t.
+    wp_pures.
+
+    destruct ok; last first.
+    { exfalso. naive_solver. }
+    apply map_get_true in HseqGet.
+    destruct Heqb as [_ HseqLe].
+
+    (* get a copy of the is_slice for the slice we're giving in reply *)
+    assert (is_Some (lastReplyMV !! args.(CPR_CID))) as [? HlastReplyMVlookup].
+    {
+      assert (args.(CPR_CID) ∈ dom (gset u64) lastSeqM).
+      { by eapply elem_of_dom_2. }
+      assert (args.(CPR_CID) ∈ dom (gset u64) lastReplyMV).
+      { rewrite -HlastReplyMVdom in H1. done. }
+      apply elem_of_dom.
+      done.
+    }
+
+    iDestruct (big_sepM2_lookup_iff with "HlastReply_structs") as %Hdom.
+    assert (is_Some (lastReplyM !! args.(CPR_CID))) as [? HlastReplyMlookup].
+    { apply Hdom. naive_solver. }
+
+    iDestruct (big_sepM2_lookup_acc _ _ _ args.(CPR_CID) with "HlastReply_structs") as "[HlastReply_struct HlastReply_structs]".
+    {
+      done.
+    }
+    {
+      done.
+    }
+
+    iDestruct "HlastReply_struct" as (srv_val_sl ?) "[%Hx Hsrv_val_sl]".
+    assert (x = reply) as ->.
+    {
+      unfold map.map_get in HlookupReply.
+      rewrite HlastReplyMVlookup in HlookupReply.
+      naive_solver.
+    }
+
+    rewrite Hx.
+    Opaque typed_slice.is_slice_small. (* to split fraction *)
+    iDestruct "Hsrv_val_sl" as "[Hsrv_val_sl Hrep_val_sl]".
+    Transparent typed_slice.is_slice_small.
+    iSpecialize ("HlastReply_structs" with "[Hsrv_val_sl]").
+    {
+      iExists _, _.
+      iFrame.
+      done.
+    }
+    wp_storeField.
+    wp_storeField.
+
+    (* now split into stale/nonstale cases *)
+    destruct (Z.lt_ge_cases (int.Z args.(CPR_Seq)) (int.Z seqno)) as [Hcase|Hcase].
+    { (* Stale *)
+      iMod (smaller_seqno_stale_fact _ {| Req_CID:=_; Req_Seq:=_ |} seqno with "His_srv Hrpc") as "HH".
+      { done. }
+      { done. }
+      { done. }
+      iDestruct "HH" as "[Hrpc #Hstale]".
+      wp_loadField.
+      wp_apply (release_spec with "[-HΦ HCID HSeq HKey HExpValue_sl HNewValue_sl HErr HSucc Hrep_val_sl]").
+      {
+        iFrame "#∗".
+        iNext.
+        iExists _,_,_, _, _, _, _, _.
+        iExists _, _, _, _.
+        iFrame.
+        done.
+      }
+      iApply "HΦ".
+
+      iSplitL "HErr HSucc".
+      {
+        instantiate (1:={| CPR_Err := _ |}).
+        iFrame.
+      }
+      iLeft.
+      iFrame "#".
+    }
+    { (* Not stale *)
+      assert (seqno = args.(CPR_Seq)) by word.
+      rewrite H1 in HseqGet.
+      iMod (server_replies_to_request _ {| Req_CID:=_; Req_Seq:=_ |} with "His_srv Hrpc") as "HH".
+      { done. }
+      { done. }
+      { eexists (mkShardReplyC 0 [] false). naive_solver. }
+
+      iDestruct "HH" as "[#Hreceipt Hrpc]".
+
+      (* prove that args.(GR_CID) is in lastReplyMV (probably just add [∗ map] _ ↦ _;_ ∈ lastReplyMV ; lastSeq, True) *)
+      wp_loadField.
+      wp_apply (release_spec with "[-HΦ HCID HSeq HKey HExpValue_sl HNewValue_sl HErr HSucc Hrep_val_sl]").
+      {
+        iFrame "#∗".
+        iNext.
+        iExists _,_,_, _, _, _, _, _.
+        iExists _, _, _, _.
+        iFrame.
+        done.
+      }
+      iApply "HΦ".
+      iSplitL "HErr HSucc".
+      {
+        instantiate (1:={| CPR_Err := _ |}).
+        by iFrame.
+      }
+      iRight.
+      rewrite HlastReplyMlookup.
+      simpl.
+      destruct x0.
+      iExists _.
+      iFrame "#".
+    }
+  }
+  {
+    wp_loadField.
+    wp_loadField.
+    wp_loadField.
+    wp_apply (wp_MapInsert with "HlastSeqMap").
+    { done. }
+    iIntros "HlastSeqMap".
+
+    wp_pures.
+    wp_loadField.
+    wp_apply (wp_shardOf).
+    wp_pures.
+    wp_loadField.
+
+    iDestruct (typed_slice.is_slice_small_acc with "HshardMap_sl") as "[HshardMap_sl HshardMap_sl_close]".
+    set (sid:=shardOfC args.(CPR_Key)) in *.
+
+    assert (∃ b, shardMapping !! int.nat sid = Some b) as [? ?].
+    {
+      eapply list_lookup_lt.
+      rewrite HshardMapLength.
+      rewrite /sid /shardOfC /uNSHARD.
+      word.
+    }
+    wp_apply (typed_slice.wp_SliceGet with "[$HshardMap_sl]").
+    {
+      iPureIntro. done.
+    }
+    iIntros "HshardMap_sl".
+    wp_pures.
+
+    assert (int.Z seqno < int.Z args.(CPR_Seq))%Z as HseqFresh.
+    {
+      simpl.
+      destruct ok.
+      {
+        intuition.
+        destruct (Z.le_gt_cases (int.Z args.(CPR_Seq)) (int.Z seqno)) as [Hineq|Hineq].
+        { naive_solver. }
+        { naive_solver. }
+      }
+      {
+        apply map_get_false in HseqGet as [_ ->].
+        simpl.
+        word.
+      }
+    }
+
+    (* get resources out of escrow before splitting into cases *)
+    iMod (server_takes_request with "HreqInv Hrpc") as "HH".
+    { done. }
+    {
+      rewrite HseqGet.
+      done.
+    }
+    iDestruct "HH" as "(Hγpre & Hpre & Hproc)".
+
+    wp_if_destruct.
+    { (* have the shard *)
+      wp_loadField.
+      iDestruct (is_slice_split with "Hkvss_sl") as "[Hkvss_sl Hkvss_sl_close]".
+      iDestruct (big_sepS_elem_of_acc _ _ sid with "HownShards") as "[HownShard HownShards]".
+      { set_solver. }
+      iDestruct "HownShard" as "[%Hbad|HownShard]".
+      { exfalso. done. }
+      iDestruct "HownShard" as (kvs_ptr m mv) "(HshardGhost & %Hkvs_lookup & HkvsMap & HvalSlices)".
+      wp_apply (wp_SliceGet _ _ _ _ _ _ _ (#kvs_ptr) with "[Hkvss_sl]").
+      {
+        iFrame "Hkvss_sl".
+        iPureIntro.
+        rewrite list_lookup_fmap.
+        rewrite Hkvs_lookup.
+        done.
+      }
+      iIntros "[Hkvss_sl %Hkvs_ty]".
+
+      wp_loadField.
+      wp_apply (map.wp_MapGet with "[$HkvsMap]").
+      iIntros (value okValue) "[%HlookupVal HkvsMap]".
+      assert (value = default (slice_val Slice.nil) (mv !! args.(CPR_Key))) as ->.
+      { naive_solver. }
+      iDestruct (big_sepS_delete _ _ args.(CPR_Key) with "HvalSlices") as "[Hsrv_val_sl HvalSlices]".
+      { set_solver. }
+      iDestruct "Hsrv_val_sl" as "[%Hbad|Hsrv_val_sl]".
+      { exfalso. done. }
+      iDestruct "Hsrv_val_sl" as (curv_sl) "[%HvalSliceRe Hsrv_val_sl]".
+      rewrite HvalSliceRe.
+
+      wp_loadField.
+      wp_apply (wp_bytesEqual with "[$HExpValue_sl $Hsrv_val_sl]").
+      iIntros "[HExpValue_sl Hsrv_val_sl]".
+
+      (* Avoid duplicating the proof of the merged control flow after this if *)
+      wp_apply (wp_If_join_evar with "[HkvsMap HKey HNewValue]").
+      { iIntros (succ Hsucc).
+        case_bool_decide as Heq; wp_pures.
+        - wp_loadField.
+          wp_loadField.
+          set (old_map := (mv, _)).
+          wp_apply (map.wp_MapInsert with "[$HkvsMap]").
+          iIntros "HkvsMap".
+          wp_pures. iModIntro.
+          iSplit; first done.
+          set (new_map := map.map_insert _ args.(CPR_Key) _).
+          replace (new_map) with (if succ then new_map else old_map); last by rewrite Hsucc.
+          iNamedAccu.
+        - iModIntro. iSplit; first done.
+          rewrite Hsucc.
+          iFrame. }
+      iIntros "Hjoined". iNamed "Hjoined".
+      set (succ := bool_decide (_ = _)).
+
+      wp_storeField.
+      wp_storeField.
+      iDestruct (big_sepS_delete _ _ args.(CPR_Key) with "HshardGhost") as "[Hghost HshardGhost]".
+      { set_solver. }
+      iDestruct "Hghost" as "[%Hbad|Hkvptsto]".
+      { exfalso; done. }
+
+      (* Get Q by using fupd *)
+      unfold PreShardConditionalPut.
+      iApply ncfupd_wp.
+      iMod (ncfupd_mask_subseteq _) as "Hclose"; last iMod "Hpre".
+      { done. }
+      iDestruct "Hpre" as (v0) "(Hkvptsto2 & HfupdQ)".
+      iDestruct (kvptsto_agree with "Hkvptsto Hkvptsto2") as %<-.
+      set (newv := if succ then args.(CPR_NewValue) else (default [] (m !! args.(CPR_Key)))).
+      iMod (kvptsto_update newv with "Hkvptsto Hkvptsto2") as "[Hkvptsto Hkvptsto2]".
+      iMod ("HfupdQ" with "Hkvptsto") as "Q".
+      iMod "Hclose" as "_".
+
+      (* fill in reply struct *)
+      iModIntro.
+      wp_loadField.
+      wp_loadField.
+      wp_loadField.
+      wp_loadField.
+
+      (* save reply in reply table *)
+      Transparent struct.load.
+      unfold struct.load.
+
+      wp_apply (map.wp_MapInsert with "HlastReplyMap").
+      iIntros "HlastReplyMap".
+
+      wp_pures.
+
+      iMod (server_completes_request with "His_srv HreqInv Hγpre [Q] Hproc") as "HH".
+      { done. }
+      { done. }
+      { rewrite HseqGet. simpl. done. }
+      {
+        iNext.
+        iRight.
+        iFrame.
+        instantiate (1:=mkShardReplyC _ [] succ).
+        simpl.
+        eauto.
+      }
+      iDestruct "HH" as "(#Hreceipt & Hrpc)".
+
+      iDestruct ("HshardMap_sl_close" with "HshardMap_sl") as "HshardMap_sl".
+      wp_loadField.
+      wp_apply (release_spec with "[-HΦ HCID HSeq HKey HErr HSucc]").
+      {
+        iFrame "HmuInv Hlocked".
+        iNext.
+        iExists _,_,_, _, _, _, _, _.
+        iExists _, _, _, _.
+        iFrame.
+        iSplitL "".
+        {
+          iPureIntro.
+          simpl.
+          rewrite !dom_insert_L.
+          congruence.
+        }
+        iSplitL "HlastReply_structs".
+        {
+          iApply (big_sepM2_insert_2 with "[] HlastReply_structs").
+          { simpl.
+            iExists _, 1%Qp.
+            rewrite zero_slice_val.
+            iSplitL ""; first done.
+            iApply (typed_slice.is_slice_small_nil).
+            done.
+          }
+        }
+        iSplitL ""; first done.
+        iSplitL ""; first done.
+        iApply "HownShards".
+        iRight.
+        iExists _, _, _.
+        iFrame.
+        instantiate (1:=(<[args.(CPR_Key):=newv]> m)).
+        iSplitL "HshardGhost Hkvptsto2".
+        {
+          iApply (big_sepS_delete _ _ args.(CPR_Key) with "[-]").
+          { set_solver. }
+          iSplitL "Hkvptsto2".
+          {
+            iRight.
+            rewrite lookup_insert.
+            iFrame.
+          }
+          iApply (big_sepS_impl with "HshardGhost").
+          iModIntro; iIntros.
+          rewrite lookup_insert_ne; last first.
+          { set_solver. }
+          iFrame.
+        }
+        iSplitL ""; first done.
+        iSplitL "HkvsMap".
+        { instantiate (1:=if succ then _ else _).
+          destruct succ; done. }
+        iApply (big_sepS_delete _ _ args.(CPR_Key) with "[-]").
+        { set_solver. }
+        simpl. iSplitL "HNewValue_sl Hsrv_val_sl".
+        {
+          simpl. iRight. destruct succ.
+          - iExists newv_sl.
+            rewrite lookup_insert.
+            rewrite lookup_insert.
+            iSplitL ""; first done.
+            iFrame.
+          - iExists curv_sl.
+            rewrite lookup_insert.
+            iSplitL ""; first done.
+            iFrame.
+        }
+        iApply (big_sepS_impl with "HvalSlices").
+        iModIntro.
+        iIntros.
+        rewrite lookup_insert_ne; last first.
+        { set_solver. }
+        destruct succ.
+        - rewrite lookup_insert_ne; last first.
+          { set_solver. }
+          iFrame.
+        - iFrame.
+      }
+      iApply "HΦ".
+      iSplitL "HErr HSucc".
+      {
+        instantiate (1:=mkConditionalPutReplyC _ _).
+        iFrame.
+      }
+      iSimpl.
+      iRight.
+      iExists [].
+      iFrame "#".
+    }
+    { (* don't have shard *)
+      wp_storeField.
+
+      iMod (server_completes_request with "His_srv HreqInv Hγpre [Hpre] Hproc") as "HH".
+      { done. }
+      { done. }
+      { rewrite HseqGet. simpl. done. }
+      {
+        iNext.
+        iLeft.
+        iFrame "Hpre".
+        instantiate (1:=mkShardReplyC 1 [] _).
+        simpl.
+        done.
+      }
+      iDestruct "HH" as "(#Hreceipt & Hrpc)".
+
+      Transparent struct.load.
+      unfold struct.load.
+      wp_loadField.
+      wp_loadField.
+      wp_loadField.
+      wp_loadField.
+      rewrite zero_slice_val.
+
+      wp_apply (map.wp_MapInsert with "HlastReplyMap").
+      iIntros "HlastReplyMap".
+      wp_pures.
+
+      wp_loadField.
+      iSpecialize ("HshardMap_sl_close" with "HshardMap_sl").
+      wp_apply (release_spec with "[-HΦ HCID HSeq HKey HErr HSucc]").
+      {
+        iFrame "HmuInv Hlocked".
+        iNext.
+        iExists _,_,_, _, _, _, _, _.
+        iExists _, _, _, _.
+        iFrame.
+        iSplitL "".
+        { iPureIntro.
+          rewrite !dom_insert_L /=.
+          congruence. }
+        iSplitL "HlastReply_structs".
+        {
+          iApply (big_sepM2_insert_2 with "[] HlastReply_structs").
+          simpl.
+          iExists Slice.nil, 1%Qp; iFrame.
+          iSplitL ""; first done.
+          iApply (typed_slice.is_slice_small_nil).
+          done.
+        }
+        done.
+      }
+      iApply "HΦ".
+      iSplitL "HErr HSucc".
+      {
+        instantiate (1:=mkConditionalPutReplyC _ _).
+        iFrame.
+      }
+      iSimpl.
+      iRight.
+      iExists []; iFrame "Hreceipt".
+    }
+  }
+Qed.
+
+End memkv_conditional_put_proof.
+
+Ltac Zify.zify_post_hook ::= idtac.
